memory safety for Exponentiation?

code/experimental/rsa/Exponentiation.fst
@@ -18,6 +18,33 @@ type lbignum (len:U32.t) =
 
 type bnlen = (l:U32.t{U32.v l > 0 /\ U32.v l <= 8192})
 
+type exp_state (rLen:bnlen) (aLen:bnlen) = lbignum U32.(rLen +^ aLen +^ (aLen +^ aLen) +^ (rLen +^ aLen))
+
+let get_acc #r #a (st:exp_state r a) : lbignum r = Buffer.sub st 0ul r
+let get_a_1 #r #a (st:exp_state r a) : lbignum a = Buffer.sub st r a
+let get_a2 #r #a (st:exp_state r a) : lbignum U32.(a +^ a) = Buffer.sub st U32.(r +^ a) U32.(a +^ a)
+let get_acc2 #r #a (st:exp_state r a) :lbignum U32.(a +^ r) = Buffer.sub st U32.(r +^ a +^ (a +^ a)) U32.(r +^ a)
+
+let exp_state_inv r a (st:exp_state r a) = 
+           let acc = get_acc st in
+           let a = get_a_1 st in
+           let a2 = get_a2 st in
+           let acc2 = get_acc2 st in
+           let r = frameOf acc in
+	     r == frameOf a /\
+	     r == frameOf a2 /\
+	     r == frameOf acc2 /\
+	     disjoint acc a /\
+	     disjoint acc a2 /\
+	     disjoint acc acc2 /\ 
+	     disjoint a a2 /\ 
+	     disjoint a acc2 /\ 
+       	 disjoint acc2 a2 
+
+
+let exp_state_st_inv (rLen:bnlen) (aLen:bnlen) (st:exp_state rLen aLen) (h:FStar.HyperStack.mem) = 
+	     exp_state_inv rLen aLen st /\ live h st
+
 (* check if input[ind] is equal to 1 *)
 val bn_bit_is_set:
     input:bignum -> 
@@ -38,38 +65,37 @@ val mod_exp_loop:
     modBits:U32.t{U32.v modBits > 0} -> aLen:bnlen ->
     bBits:U32.t{U32.v bBits > 0} -> resLen:bnlen ->
     n:lbignum (bits_to_bn modBits) ->
-    a:lbignum aLen ->
     b:lbignum (bits_to_bn bBits) ->
-    acc:lbignum resLen ->
+    st:exp_state resLen aLen{disjoint st n /\ disjoint st b} ->
     count:U32.t{U32.v count <= U32.v bBits} -> Stack unit
-    (requires (fun h -> live h n /\ live h a /\ live h b /\ live h acc))
-    (ensures  (fun h0 _ h1 -> live h0 n /\ live h0 a /\ live h0 b /\ live h0 acc /\
-        live h1 n /\ live h1 a /\ live h1 b /\ live h1 acc /\
-        modifies_2 a acc h0 h1))
+    (requires (fun h -> live h n /\ live h b /\ exp_state_st_inv resLen aLen st h))
+    (ensures  (fun h0 _ h1 -> live h1 n /\ live h1 b /\ exp_state_st_inv resLen aLen st h1 /\
+                modifies_1 st h0 h1))
 
-let rec mod_exp_loop modBits aLen bBits resLen n a b acc count =
-    push_frame();
+#set-options "--z3rlimit 150 --max_fuel 2"
+
+let rec mod_exp_loop modBits aLen bBits resLen n b st count =
+    let acc = get_acc st in
+    let a = get_a_1 st in
+    let a2 = get_a2 st in
+    let acc2 = get_acc2 st in
     let a2Len = U32.(aLen +^ aLen) in
     let acc2Len = U32.(resLen +^ aLen) in
-    let a2 = create 0uL a2Len in
-    let acc2 = create 0uL acc2Len in
-    let a2_r = create 0uL aLen in
+    fill a2 0uL a2Len;
+    fill acc2 0uL acc2Len;
 
-    let diffBits1 = U32.(64ul *^ a2Len -^ modBits) in
-    let diffBits2 = U32.(64ul *^ acc2Len -^ modBits) in
+    let diffBits1 = U32.(64ul *^ a2Len -%^ modBits) in
+    let diffBits2 = U32.(64ul *^ acc2Len -%^ modBits) in
     let modLen = bits_to_bn modBits in
-
     (if U32.(count <^ bBits) then begin
         sqr aLen a a2;
-        Div.remainder a2Len modLen aLen diffBits1 a2 n a2_r;
+        Div.remainder a2Len modLen aLen diffBits1 a2 n a;
         (if (bn_bit_is_set b count) then begin
-            mult resLen aLen acc a2_r acc2;
+            mult resLen aLen acc a acc2;
             Div.remainder acc2Len modLen resLen diffBits2 acc2 n acc
         end);
-        blit a2_r 0ul a 0ul aLen;
-        mod_exp_loop modBits aLen bBits resLen n a b acc U32.(count +^ 1ul)
-    end);
-    pop_frame()
+        mod_exp_loop modBits aLen bBits resLen n b st U32.(count +^ 1ul)
+    end)
 
 (* res = a ^^ b mod n *)
 val mod_exp:
@@ -84,16 +110,19 @@ val mod_exp:
         live h1 n /\ live h1 a /\ live h1 b /\ live h1 res /\
         modifies_1 res h0 h1))
 
+#set-options "--z3rlimit 150 --max_fuel 0"
+
 let mod_exp modBits aLen bBits resLen n a b res =
     push_frame();
-    let acc = create 0uL resLen in
-    let a_1 = create 0uL aLen in
+    let st : exp_state resLen aLen = create 0uL U32.(resLen +^ aLen +^ (aLen +^ aLen) +^ (resLen +^ aLen)) in
+    let acc = get_acc st in
+    let a_1 = get_a_1 st in
     blit a 0ul a_1 0ul aLen;
 
     (if (bn_bit_is_set b 0ul) then
         blit a_1 0ul acc 0ul aLen
     else acc.(0ul) <- 1uL);
 
-    mod_exp_loop modBits aLen bBits resLen n a_1 b acc 1ul;
+    mod_exp_loop modBits aLen bBits resLen n b st 1ul;
     blit acc 0ul res 0ul resLen;
     pop_frame()
